build split function without body

KmsArnIdeGen3.dfy
@@ -1,43 +1,43 @@
-predicate ArnString?(s: string)
-{
-    s == "arn"
-}
-// MUST start with string arn
-type ArnString = s:string |  s == "arn" witness *
+// predicate ArnString?(s: string)
+// {
+//     s == "arn"
+// }
+// // MUST start with string arn
+// type ArnString = s:string |  s == "arn" witness *
 
 
-// The partition MUST be a non-empty
-predicate PartitionString?(s:string)
-{
-    |s|!=0
-}
-type PartitionString = s:string | PartitionString?(s) witness *
+// // The partition MUST be a non-empty
+// predicate PartitionString?(s:string)
+// {
+//     |s|!=0
+// }
+// type PartitionString = s:string | PartitionString?(s) witness *
 
 
 
-// The service MUST be the string kms
-predicate ServiceString?(s:string)
-{
-    |s|!=0
-}
+// // The service MUST be the string kms
+// predicate ServiceString?(s:string)
+// {
+//     |s|!=0
+// }
 
-type ServiceString = s | ServiceString?(s) witness *
+// type ServiceString = s | ServiceString?(s) witness *
 
-// The region MUST be a non-empty string
-predicate RegionString?(s:string)
-{
-    |s|!=0
-}
-type RegionString = s:string | RegionString?(s) witness *
+// // The region MUST be a non-empty string
+// predicate RegionString?(s:string)
+// {
+//     |s|!=0
+// }
+// type RegionString = s:string | RegionString?(s) witness *
 
-//The account MUST be a non-empty string
-predicate AccountString?(s:string)
-{
-    |s|!=0
+// //The account MUST be a non-empty string
+// predicate AccountString?(s:string)
+// {
+//     |s|!=0
 
-}
+// }
 
-type AccountString = s:string | AccountString?(s) witness *
+// type AccountString = s:string | AccountString?(s) witness *
 
 
 datatype Resource = Resource(
@@ -46,11 +46,11 @@ datatype Resource = Resource(
 )
 
 datatype ARN = ARN(
-    arnLiteral: ArnString,
-    partition: PartitionString,
-    service: ServiceString,
-    region: RegionString,
-    account: AccountString,
+    arnLiteral: string,
+    partition: string,
+    service: string,
+    region: string,
+    account: string,
     resource: Resource
 )
 
@@ -107,10 +107,37 @@ function method AwsKmsMrkArnIdentifier(a:string) : bool
     if "arn:" < a 
     then true // AwsKmsMrkArn's input is not a string yet, we'll fill in later
     else "mrk-" < a
+
+}
+
+function method splitArnString(s:string, delimiter:char):(output:seq<string>)
+    requires multiset(s)[delimiter] == 5
+    requires multiset(s)['/'] == 1
+    ensures |output| == 5
+    
+    
+    
+
+
+function method splictArnResourceString (s:string):(output:seq<string>)
+    requires multiset(s)['/'] == 2
+    ensures |output| == 2
+
+
+
+function method createArn(a:seq<string>):ARN
+    requires |a| == 6 && multiset(a[5])['/'] == 2
+    requires ARN(a[0], a[1], a[2], a[3], a[4], Resource(splictArnResourceString(a[5])[0],splictArnResourceString(a[5])[1])).ARN?
+    requires multiset(a[5])['/'] == 2
+{   
+    var resourceSeq := splictArnResourceString(a[5]);    
+    ARN(a[0], a[1], a[2], a[3], a[4], Resource(resourceSeq[0],resourceSeq[1]))
 }
 
 
-lemma  asdf(a: ARN)
+
+
+lemma asdf(a: ARN)
     requires KmsArn?(a)
     ensures AwsKmsMrkArn(a).Success?
 {
